ulib/Test.Vale.fst
@@ -1,0 +1,55 @@
+module Test.Vale
+
+open FStar.Heap
+open FStar.Heap.Vale
+
+(*
+ * test the model
+ *)
+let test (m0:mem{sync m0}) =
+  let href, m1 = alloc #Bool m0 true in  //allocate a boolean value
+
+  let a = get_lo_start m1 (addr_of href) in  //a is the address in the lo-level view
+
+  (* check that the lo-level view is correct and that m1 is synchronized *)
+  assert (load m1 a = b1);
+  ()
+
+
+  assert (sync m1);
+
+  (* update the hi-level heap, and check that the updates are reflected in the lo-level view *)
+  let m2 = upd m1 href false in
+  assert (load m2 a = b0);
+  assert (sync m2);
+
+  (* update the lo-level view and check that the updates are reflected in the hi-level view *)
+  let m3 = store m2 a b1 in
+  assert (sel m3 href = true);
+  assert (sync m3);
+
+  (* store a bad value in the lo-level, check that the hi-level view is unchanged and the mem is no longer synchronized *)
+  let m4 = store m3 a b2 in
+  assert (sel m4 href = true);
+  assert (~ (sync m4));
+
+  (* store back a good value, and check that the hi-level view is again in sync *)
+  let m5 = store m4 a b0 in
+  assert (sel m5 href = false);
+  assert (sync m5);
+
+  let href1, m6 = alloc #Bool m5 true in
+  let a1 = get_lo_start m6 (addr_of href1) in
+
+  assert (addr_of href =!= addr_of href1);
+
+  assert (sel m6 href == false);
+  assert (load m6 a1 == b1);
+
+  let m7 = store m6 a1 b1 in
+
+  assert (sel m7 href1 == true);
+  assert (sel m7 href == false);
+  assert (load m7 a == b0);
+
+  ()
